- Math_BarycentricInterpolation_1
```math
\alpha + \beta + \gamma = 1
```

- Math_BarycentricInterpolation_2
```math
(\alpha + \beta + \gamma)v_P = \alpha v_A + \beta v_B + \gamma v_C
```

- Math_BarycentricInterpolation_3
```math
S_{\Delta PAB} = \frac{|\overrightarrow{PA}||\overrightarrow{PB}|\sin (\theta_1)}{2}
```

- Math_BarycentricInterpolation_4
```math
|\overrightarrow{PA}| = \sqrt{(x_A - x_P) ^2 + (y_A - y_P) ^2}
```

- Math_BarycentricInterpolation_5
```math
|\overrightarrow{PB}| = \sqrt{(x_B - x_P) ^2 + (y_B - y_P) ^2}
```

- Math_BarycentricInterpolation_6
```math
\sin (\theta_{PAB}) =\sqrt{1 - (\frac{\overrightarrow{PA} \cdot\overrightarrow{PB}}{|\overrightarrow{PA}||\overrightarrow{PB}|})^2 }     
```

- Math_BarycentricInterpolation_7
```math
S_{\Delta PAB} = \frac{(x_A - x_P)(y_B - y_P) - (x_B - x_P)(y_A - y_P)}{2}
```

- Math_BarycentricInterpolation_8
```math
S_{\Delta PBC} = \frac{(x_B - x_P)(y_C - y_P) - (x_C - x_P)(y_B - y_P)}{2}
```

- Math_BarycentricInterpolation_9
```math
S_{\Delta PCA} = \frac{(x_C - x_P)(y_A - y_P) - (x_A - x_P)(y_C - y_P)}{2}
```

- Math_BarycentricInterpolation_10
```math
S_{\Delta CAB} = \frac{(x_A - x_C)(y_B - y_C) - (x_B - x_C)(y_A - y_C)}{2}
```

- Math_BarycentricInterpolation_11
```math
\alpha = \frac{(x_B - x_P)(y_C - y_P) - (x_C - x_P)(y_B - y_P)}{(x_A - x_C)(y_B - y_C) - (x_B - x_C)(y_A - y_C)}
```

- Math_BarycentricInterpolation_12
```math
\beta = \frac{(x_C - x_P)(y_A - y_P) - (x_A - x_P)(y_C - y_P)}{(x_A - x_C)(y_B - y_C) - (x_B - x_C)(y_A - y_C)}
```

- Math_BarycentricInterpolation_13
```math
\gamma = \frac{(x_A - x_P)(y_B - y_P) - (x_B - x_P)(y_A - y_P)}{(x_A - x_C)(y_B - y_C) - (x_B - x_C)(y_A - y_C)}
```

- Math_BarycentricInterpolation_14
```math
ax + bz = c
```

- Math_BarycentricInterpolation_15
```math
\frac{x_{A'}}{x_A} = \frac{z_{A'}}{-n}
```

- Math_BarycentricInterpolation_16
```math
\frac{1}{z_{A'}} = -\frac{ax_{A}}{cn} + \frac{b}{c}
```

- Math_BarycentricInterpolation_17
```math
\frac{1}{z'} = -\frac{ax}{cn} + \frac{b}{c}
```

- Math_BarycentricInterpolation_18
```math
P = (1 - t) A + t B
```

- Math_BarycentricInterpolation_19
```math
\frac{1}{z_{P'}} = -\frac{ax_P}{cn} + \frac{b}{c}
```

- Math_BarycentricInterpolation_20
```math
\frac{1}{z_{P'}} = -\frac{ax_A}{cn}(1 - t) - \frac{ax_B}{cn}t + \frac{b}{c}
```

- Math_BarycentricInterpolation_21
```math
\frac{1}{z_{P'}} = (-\frac{ax_A}{cn}(1 - t) + \frac{b}{c}(1 - t)) + (-\frac{ax_B}{cn}t + \frac{b}{c}t)
```

- Math_BarycentricInterpolation_21
```math
\frac{1}{z_{P'}} = \frac{1}{z_A}(1 - t) + \frac{1}{z_B}t
```

- Math_BarycentricInterpolation_22
```math
ax + by + cz = d 
```

- Math_BarycentricInterpolation_23
```math
\frac{x_{A'}}{x_A} = \frac{z_{A'}}{-n}
```

- Math_BarycentricInterpolation_24
```math
\frac{y_{A'}}{y_A} = \frac{z_{A'}}{-n}
```

- Math_BarycentricInterpolation_25
```math
\frac{1}{z_{A'}} = -\frac{ax_A}{dn} - \frac{by_A}{dn} + \frac{c}{d}
```

- Math_BarycentricInterpolation_26
```math
\frac{1}{z'} = -\frac{ax}{dn} - \frac{by}{dn} + \frac{c}{d}
```

- Math_BarycentricInterpolation_27
```math
P = \alpha A + \beta B + \gamma C
```

- Math_BarycentricInterpolation_28
```math
\alpha + \beta + \gamma = 1
```

- Math_BarycentricInterpolation_29
```math
\frac{1}{z_{P'}} = -\frac{ax_P}{dn} - \frac{by_P}{dn} + \frac{c}{d}
```

- Math_BarycentricInterpolation_30
```math
x_P = \alpha x_A + \beta x_B + \gamma x_C
```

- Math_BarycentricInterpolation_31
```math
y_P = \alpha y_A + \beta y_B + \gamma y_C
```

- Math_BarycentricInterpolation_32
```math
\frac{1}{z_{P'}} = \alpha(-\frac{ax_A}{dn} - \frac{by_A}{dn} + \frac{c}{d}) + \beta(-\frac{ax_B}{dn} - \frac{by_B}{dn} + \frac{c}{d}) + \gamma(-\frac{ax_C}{dn} - \frac{by_C}{dn} + \frac{c}{d})
```

- Math_BarycentricInterpolation_33
```math
\frac{1}{z_{P'}} = \frac{1}{z_{A'}}\alpha + \frac{1}{z_{B'}}\beta + \frac{1}{z_{C'}}
```

- Math_BarycentricInterpolation_34
```math
P = \alpha A + \beta B + \gamma C = (1 - \beta - \gamma)A + \beta B + \gamma C = A + \beta\overrightarrow{AB} + \gamma\overrightarrow{AC}
```